Rewrite dataStructure (#1)
* Add random grid generation

* Add sum calculation

* Add grid changing functionality

* Add documentation

* Add game won determination

sumplete/sumplete.dfy
@@ -5,89 +5,220 @@ Project: Part 1 - Sumplete
 
 module DataStructure {
   /**
-  Sums of a grid.
-   */
-  class Sums {
-    var rows: array<int>
-    var columns: array<int>
-
-    constructor(size: nat)
-      ensures rows.Length == size
-      ensures columns.Length == size
-    {
-      rows := new int[size];
-      columns := new int[size];
-    }
-
-    method updateRows(sums: array<int>)
-      modifies this
-      requires sums.Length == rows.Length
-    {
-      rows := sums;
-    }
-
-    method updateColumns(sums: array<int>)
-      modifies this
-      requires sums.Length == columns.Length
-    {
-      columns := sums;
-    }
-
-    /*
-    function rowsMatch(playerRows: array<int>) : (matches: bool)
-      reads playerRows
-      reads this
-      requires rows.Length == playerRows.Length
-      ensures forall i | 0 <= i < rows.Length :: rows[i] == playerRows[i] ==> matches == true
-      ensures exists i | 0 <= i < rows.Length :: rows[i] != playerRows[i] ==> matches == false
-    {
-      // TODO
-    }
-    */
-  }
-
-  /**
   The sumplete grid.
    */
   class Grid {
+    // grid_size == n
+    ghost var grid_size: int
+
     // n*n grid -> rows*columns
-    var grid_start: array2<int>
-    var sum_target: Sums
+    var start_grid: array2<int> // grid that gets displayed to the player
 
-    var grid_player: array2<int>
-    var sum_player: Sums
+    var target_grid: array2<int> // solution to the puzzle
+    var target_rows_sum: array<int> // rows sums the player has to fulfill
+    var target_columns_sum: array<int> // column sums the player has to fulfill
 
-    constructor(grid: array2<int>)
-      requires grid.Length0 == grid.Length1
-      ensures grid_start.Length0 == grid_start.Length1
-      ensures grid_start.Length0 == grid_player.Length0
-      ensures grid_start.Length1 == grid_player.Length1
-      ensures grid_start.Length0 == sum_target.rows.Length
-      ensures grid_player.Length0 == sum_player.rows.Length
+    var player_grid: array2<int> // grid with the currently chosen numbers, at the beginning all nums are deactivated
+    var player_rows_sum: array<int> // rows sum that the player currently has
+    var player_columns_sum: array<int> // columns sum that the player currently has
+
+    /**
+    Ensures that all grids are the same size and the rows and columns have the correct sizes for the grids.
+     */
+    ghost predicate Valid()
+      reads this
     {
-      grid_start := grid;
-      grid_player := new int[grid.Length0, grid.Length1]((i, j) => 0);
+      // ensure all grids have the same n*n size
+      grid_size == start_grid.Length0 && grid_size == start_grid.Length1 &&
+      grid_size == target_grid.Length0 && grid_size == target_grid.Length1 &&
+      grid_size == player_grid.Length0 && grid_size == player_grid.Length1 &&
 
-      sum_target := new Sums(grid.Length0);
-      sum_player := new Sums(grid.Length0);
+      // ensure sum arrays have same length as rows & columns
+      grid_size == target_rows_sum.Length && grid_size == target_columns_sum.Length &&
+      grid_size == player_rows_sum.Length && grid_size == player_columns_sum.Length
     }
 
     /**
-    Sets the row or column sum.
+    Instantiates the grids and sums.
      */
-    /*
-    method setSums(rowSums: array<int>, columnSums: array<int>)
-      modifies this
-      requires rowSums.Length == sum_target.rows.Length
-      requires columnSums.Length == sum_target.columns.Length
+    constructor(size: int)
+      requires size > 0
+      ensures Valid()
     {
-      sum_target.updateRows(rowSums);
-      sum_target.updateColumns(columnSums);
-    }*/
+      grid_size := size;
+
+      start_grid := new int[size, size]((i, j) => 0);
+
+      target_grid := new int[size, size]((i, j) => 0);
+      target_rows_sum := new int[size](i => 0);
+      target_columns_sum := new int[size](i => 0);
+
+      player_grid := new int[size, size]((i, j) => 0);
+      player_rows_sum := new int[size](i => 0);
+      player_columns_sum := new int[size](i => 0);
+    }
+
+    /**
+    Sets up the game by:
+    - filling the start_grid with random numbers
+    - filling the target_grid with the chosen numbers
+    - calculating the target_(rows/columns)_sums
+     */
+    method setupGame()
+      modifies this, start_grid, target_grid, target_rows_sum, target_columns_sum
+      requires Valid()
+      ensures Valid()
+    {
+      var i, j := 0, 0;
+      var size := start_grid.Length0;
+
+      while i < size
+        invariant size == grid_size
+        invariant Valid()
+        modifies start_grid, target_grid
+      {
+        while j < size
+          invariant size == grid_size
+          invariant Valid()
+          modifies start_grid, target_grid
+        {
+          start_grid[i,j] := random();
+          var randomBool := randomBool();
+          if randomBool {
+            target_grid[i,j] := start_grid[i,j];
+          }
+          j := j + 1;
+        }
+        i := i + 1;
+      }
+
+      i, j := 0, 0;
+      while i < size
+        invariant size == grid_size
+        invariant Valid()
+        modifies target_rows_sum, target_columns_sum
+      {
+        while j < size
+          invariant size == grid_size
+          invariant Valid()
+          modifies target_rows_sum, target_columns_sum
+        {
+          var currentNum := target_grid[i,j];
+          target_rows_sum[i] := target_rows_sum[i] + currentNum;
+          target_columns_sum[j] := target_columns_sum[j] + currentNum;
+          j := j + 1;
+        }
+        i := i + 1;
+      }
+    }
+
+    /**
+    Toggles the field to a value or 0, depending on its previous value.
+    Also updates the sums and checks if the game is won.
+
+    @param{row} The row where the field is located.
+    @param{column} The column where the field is located.
+
+    @returns{bool} True if the game is won, else false.
+     */
+    method toggleField(row: nat, column: nat) returns (gameWon: bool)
+      modifies this, player_grid, player_rows_sum, player_columns_sum
+      requires Valid()
+      requires 0 <= row < grid_size && 0 <= column < grid_size
+      ensures Valid()
+      // ensures old(player_grid[row, column]) == 0 ==> player_grid[row, column] == start_grid[row, column]
+      // ensures old(player_grid[row, column]) != 0 ==> player_grid[row, column] == 0
+    {
+      if player_grid[row, column] == 0 {
+        player_grid[row, column] := player_grid[row, column];
+      }
+      else {
+        player_grid[row, column] := 0;
+      }
+
+      calculateCurrentPlayerSums();
+      gameWon := determineGameState();
+    }
+
+    /**
+    Calculates the current sum of each player_(rows/columns)_sum.
+     */
+    method calculateCurrentPlayerSums()
+      modifies this, player_rows_sum, player_columns_sum
+      requires Valid()
+      ensures Valid()
+    {
+      var i, j := 0, 0;
+      var size := player_grid.Length0;
+
+      while i < size
+        invariant size == grid_size
+        invariant Valid()
+        modifies player_rows_sum, player_columns_sum
+      {
+        while j < size
+          invariant size == grid_size
+          invariant Valid()
+          modifies player_rows_sum, player_columns_sum
+        {
+          var currentNum := player_grid[i,j];
+          player_rows_sum[i] := player_rows_sum[i] + currentNum;
+          player_columns_sum[j] := player_columns_sum[j] + currentNum;
+          j := j + 1;
+        }
+        i := i + 1;
+      }
+    }
+
+    /**
+    Checks if game is won with the current player_grid.
+
+    @returns{bool} True if the game is won, else false.
+     */
+    method determineGameState() returns (isGameWon: bool)
+      requires Valid()
+      ensures Valid()
+    {
+      var i := 0;
+      isGameWon := true;
+
+      while i < player_rows_sum.Length
+        invariant Valid()
+      {
+        if(player_rows_sum[i] != target_rows_sum[i] ||
+           player_columns_sum[i] != target_columns_sum[i]) {
+          isGameWon := false;
+        }
+        i := i + 1;
+      }
+    }
+
+    /**
+    Random number generator.
+
+    @returns{int} Random number between 1 and 9.
+    */
+    method random() returns (randomNumber: nat)
+      ensures 1 <= randomNumber <= 9
+    {
+      var numberSet := {1, 2, 3, 4, 5, 6, 7, 8, 9};
+      randomNumber :| randomNumber in numberSet;
+    }
+
+    /**
+    Random boolean generator.
+
+    @returns{bool} Random boolean.
+    */
+    method randomBool() returns (randomBool: bool)
+    {
+      var boolSet: set<bool> := {true, false};
+      randomBool :| randomBool in boolSet;
+    }
   }
 }
 
-module GameSetup {
+module Game {
   import dataStructure = DataStructure
 
   /**
@@ -96,70 +227,6 @@ module GameSetup {
   method setupGame(size: nat) returns (grid: dataStructure.Grid)
     requires size > 0
   {
-    var newGrid := createRandomGridOfSize(size);
-    grid := new dataStructure.Grid(newGrid);
-
-    var solutionGrid := createRandomSolutionGrid(newGrid);
-  }
-
-  /**
-  Creates a grid of size, with random numbers in every cell.
-   */
-  method createRandomGridOfSize(size: nat) returns (grid: array2<int>)
-    ensures grid.Length0 == grid.Length1
-  {
-    grid := new int[size, size]((i, j) => 0);
-
-    var i := 0;
-    var j := 0;
-    while i < grid.Length0 {
-      while j < grid.Length1 {
-        grid[i,j] := random();
-        j := j+1;
-      }
-      i := i+1;
-    }
-  }
-
-  /**
-  Creates a grid that only includes the numbers that should be counted to the column and row sums.
-   */
-  method createRandomSolutionGrid(grid: array2<int>) returns (solutionGrid: array2<int>)
-  {
-    solutionGrid := new int[grid.Length0, grid.Length1]((i, j) => 0);
-    var i := 0;
-    var j := 0;
-    var shouldBeCounted := false;
-    while i < solutionGrid.Length0 {
-      while j < solutionGrid.Length1 {
-        shouldBeCounted := randomBool();
-        if shouldBeCounted {
-          solutionGrid[i,j] := grid[i,j];
-        } else {
-          solutionGrid[i,j] := 0;
-        }
-        j := j+1;
-      }
-      i := i+1;
-    }
-  }
-
-  /**
-  Random number generator.
-   */
-  method random() returns (randomNumber: nat)
-    ensures 1 <= randomNumber <= 9
-  {
-    var numberSet := {1, 2, 3, 4, 5, 6, 7, 8, 9};
-    randomNumber :| randomNumber in numberSet;
-  }
-
-  /**
-  Random boolean generator.
-   */
-  method randomBool() returns (randomBool: bool)
-  {
-    var bools: set<bool> := {true, false};
-    randomBool :| randomBool in bools;
+    grid := new dataStructure.Grid(size);
   }
 }
